zoo_parabs/ws_deques_private: Introduce assertions and start verification.

theories/zoo_parabs/ws_deques_private.v
@@ -1,5 +1,12 @@
 From zoo Require Import
   prelude.
+From zoo.common Require Import
+  countable.
+From zoo.iris.bi Require Import
+  big_op.
+From zoo.iris.base_logic Require Import
+  lib.ghost_pred
+  lib.ghost_list.
 From zoo.language Require Import
   notations.
 From zoo.diaframe Require Import
@@ -7,90 +14,356 @@ From zoo.diaframe Require Import
 From zoo_std Require Import
   option
   array
+  atomic_array
   deque
   random_round.
 From zoo_parabs Require Export
   base
   ws_deques_private__code.
+From zoo_parabs Require Import
+  ws_deques_private__types.
 From zoo Require Import
   options.
 
-Implicit Types v t round : val.
-Implicit Types vs : list val.
-Implicit Types vss : list (list val).
+Implicit Types l : location.
+Implicit Types v t deque round : val.
+Implicit Types o : option val.
+Implicit Types vs ws : list val.
+Implicit Types vss wss : list (list val).
 Implicit Types status : status.
+Implicit Types statuses : list status.
 
 Class WsDequesPrivateG Σ `{zoo_G : !ZooG Σ} := {
+  #[local] ws_deques_private_G_models_G :: GhostListG Σ (list val) ;
+  #[local] ws_deques_private_G_channels_G :: GhostPredG Σ (option val) ;
 }.
 
 Definition ws_deques_private_Σ := #[
+  ghost_list_Σ (list val) ;
+  ghost_pred_Σ (option val)
 ].
 #[global] Instance subG_ws_deques_private_Σ Σ `{zoo_G : !ZooG Σ} :
   subG ws_deques_private_Σ Σ →
   WsDequesPrivateG Σ.
 Proof.
-  (* solve_inG. *)
+  solve_inG.
 Qed.
+
+#[local] Coercion status_to_val status : val :=
+  match status with
+  | Blocked =>
+      §Blocked
+  | Nonblocked =>
+      §Nonblocked
+  end.
+
+Inductive request :=
+  | RequestBlocked
+  | RequestNone
+  | RequestSome (i : nat).
+Implicit Types request : request.
+Implicit Types requests : list request.
+
+#[local] Coercion request_to_val request : val :=
+  match request with
+  | RequestBlocked =>
+      §RequestBlocked
+  | RequestNone =>
+      §RequestNone
+  | RequestSome i =>
+      ‘RequestSome( #i )
+  end.
+
+Inductive response :=
+  | ResponseWaiting
+  | ResponseNone
+  | ResponseSome v.
+Implicit Types response : response.
+Implicit Types responses : list response.
+
+#[local] Coercion response_to_val response : val :=
+  match response with
+  | ResponseWaiting =>
+      §ResponseWaiting
+  | ResponseNone =>
+      §ResponseNone
+  | ResponseSome v =>
+      ‘ResponseSome( v )
+  end.
 
 Section ws_deques_private_G.
   Context `{ws_deques_private_G : WsDequesPrivateG Σ}.
 
-  (* #[local] Definition ws_deques_private_inv_inner deques v_flags v_requests v_responses sz : iProp Σ := *)
-  (*   ∃ flags requests responses vss, *)
-  (*   array_model v_flags (DfracOwn 1) flags ∗ *)
-  (*   array_model v_requests (DfracOwn 1) requests ∗ *)
-  (*   array_model v_reponses (DfracOwn 1) responses ∗ *)
-  (*   ( [∗ list] deque; vs ∈ deques; vss, *)
-  (*     deque_model deque vs *)
-  (*   ) ∗ *)
-  (*   ( [∗ list] flag; vs ∈ flags; vss, *)
-  (*     ⌜flag = #(bool_decide (vs ≠ []))⌝ *)
-  (*     ⌜flag = #true ∨ flag = #false ∧ vs = []⌝ *)
-  (*   ) *)
-  (* . *)
-  (* Definition ws_deques_private_inv t ι sz : iProp Σ := *)
-  (*   ∃ deques flags requests responses, *)
-  (*   ⌜t = (v_deques, v_flags, v_requests, v_responses)%V⌝ ∗ *)
-  (*   array_model v_deques DfracDiscarded deques ∗ *)
-  (*   inv ι (ws_deques_private_inv_inner deques v_flags v_requests v_responses sz). *)
+  Implicit Types Ψ : option val → iProp Σ.
 
-  Definition ws_deques_private_inv t (ι : namespace) (sz : nat) : iProp Σ.
-  Proof. Admitted.
+  Record metadata := {
+    metadata_deques_array : val ;
+    metadata_deques : list val ;
+    metadata_statuses_array : val ;
+    metadata_requests_array : val ;
+    metadata_responses_array : val ;
+    metadata_inv : namespace ;
+    metadata_models : gname ;
+    metadata_channels : list gname ;
+  }.
+  Implicit Types γ : metadata.
+  Implicit Types γ_channels : list gname.
 
-  Definition ws_deques_private_model t vss : iProp Σ.
-  Proof. Admitted.
+  #[local] Instance metadata_eq_dec : EqDecision metadata :=
+    ltac:(solve_decision).
+  #[local] Instance metadata_countable :
+    Countable metadata.
+  Proof.
+    solve_countable.
+  Qed.
 
-  Definition ws_deques_private_owner t (i : nat) status : iProp Σ.
-  Proof. Admitted.
+  #[local] Definition models_auth' :=
+    ghost_list_auth.
+  #[local] Definition models_auth γ :=
+    models_auth' γ.(metadata_models).
+  #[local] Definition models_at' γ_models i :=
+    ghost_list_at γ_models i (DfracOwn 1).
+  #[local] Definition models_at γ :=
+    models_at' γ.(metadata_models).
+
+  #[local] Definition channels_at' γ_channels i q Ψ : iProp Σ :=
+    ∃ γ_channel,
+    ⌜γ_channels !! i = Some γ_channel⌝ ∗
+    ghost_pred γ_channel (DfracOwn q) Ψ.
+  #[local] Definition channels_at γ :=
+    channels_at' γ.(metadata_channels).
+  #[local] Instance : CustomIpatFormat "channels_at" :=
+    "(
+      %γ_channel &
+      %Hlookup &
+      Hγ_channel
+    )".
+
+  #[local] Definition request_au γ j Ψ : iProp Σ :=
+    AU <{
+      ∃∃ vss,
+      models_auth γ vss
+    }> @ ⊤ ∖ ↑γ.(metadata_inv), ∅ <{
+      ∀∀ o,
+      match o with
+      | None =>
+          models_auth γ vss
+      | Some v =>
+          ∃ vs,
+          ⌜vss !! j = Some (v :: vs)⌝ ∗
+          models_auth γ (<[j := vs]> vss)
+      end
+    , COMM
+      Ψ o
+    }>.
+
+  #[local] Definition inv_inner γ : iProp Σ :=
+    ∃ statuses requests responses,
+    array_model γ.(metadata_statuses_array) (DfracOwn 1) (status_to_val <$> statuses) ∗
+    array_model γ.(metadata_requests_array) (DfracOwn 1) (request_to_val <$> requests) ∗
+    array_model γ.(metadata_responses_array) (DfracOwn 1) (response_to_val <$> responses) ∗
+    ( [∗ list] i ↦ request ∈ requests,
+      if request is RequestSome j then
+        ∃ Ψ,
+        channels_at γ j (1/2) Ψ ∗
+        request_au γ j Ψ
+      else
+        True
+    ) ∗
+    ( [∗ list] i ↦ response ∈ responses,
+      match response with
+      | ResponseWaiting =>
+          True
+      | ResponseNone =>
+          ∃ Ψ,
+          channels_at γ i (1/2) Ψ ∗
+          Ψ None
+      | ResponseSome v =>
+          ∃ Ψ,
+          channels_at γ i (1/2) Ψ ∗
+          Ψ (Some v)
+      end
+    ).
+  #[local] Instance : CustomIpatFormat "inv_inner" :=
+    "(
+      %statuses &
+      %requests &
+      %responses &
+      >Hstatuses_model &
+      Hrequests_model &
+      Hresponses_model &
+      Hrequests &
+      Hresponses
+    )".
+  Definition ws_deques_private_inv t ι (sz : nat) : iProp Σ :=
+    ∃ l γ,
+    ⌜t = #l⌝ ∗
+    ⌜ι = γ.(metadata_inv)⌝ ∗
+    meta l nroot γ ∗
+    l.[size] ↦□ #sz ∗
+    l.[deques] ↦□ γ.(metadata_deques_array) ∗
+    ⌜length γ.(metadata_deques) = sz⌝ ∗
+    array_model γ.(metadata_deques_array) DfracDiscarded γ.(metadata_deques) ∗
+    l.[statuses] ↦□ γ.(metadata_statuses_array) ∗
+    array_inv γ.(metadata_statuses_array) sz ∗
+    l.[requests] ↦□ γ.(metadata_requests_array) ∗
+    array_inv γ.(metadata_requests_array) sz ∗
+    l.[responses] ↦□ γ.(metadata_responses_array) ∗
+    array_inv γ.(metadata_responses_array) sz ∗
+    inv ι (inv_inner γ).
+  #[local] Instance : CustomIpatFormat "inv" :=
+    "(
+      %l{} &
+      %γ{} &
+      {%Ht_eq{}=->} &
+      {%Hι_eq{}=->} &
+      #Hmeta{_{}} &
+      #Hl{}_size &
+      #Hl{}_deques &
+      %Hdeques{}_length &
+      #Hdeques{}_model &
+      #Hl{}_statuses &
+      #Hstatuses{}_inv &
+      #Hl{}_requests &
+      #Hrequests{}_inv &
+      #Hl{}_responses &
+      #Hresponses{}_inv &
+      #Hinv{}
+    )".
+
+  Definition ws_deques_private_model t vss : iProp Σ :=
+    ∃ l γ,
+    ⌜t = #l⌝ ∗
+    meta l nroot γ ∗
+    models_auth γ vss.
+  #[local] Instance : CustomIpatFormat "model" :=
+    "(
+      %l{} &
+      %γ{} &
+      %Heq{} &
+      #Hmeta{_{}} &
+      Hmodels_auth
+    )".
+
+  Definition ws_deques_private_owner t i status ws : iProp Σ :=
+    ∃ l γ deque vs Ψ,
+    ⌜t = #l⌝ ∗
+    meta l nroot γ ∗
+    ⌜γ.(metadata_deques) !! i = Some deque⌝ ∗
+    deque_model deque vs ∗
+    models_at γ i ws ∗
+    ⌜vs `suffix_of` ws⌝ ∗
+    channels_at γ i 1 Ψ.
+  #[local] Instance : CustomIpatFormat "owner" :=
+    "(
+      %l{=_} &
+      %γ{=_} &
+      %deque{} &
+      %vs{=_} &
+      %Ψ{} &
+      %Heq{} &
+      #Hmeta_{} &
+      %Hdeques_lookup{_{}} &
+      Hdeque_model{_{}} &
+      Hmodels_at{_{}} &
+      %Hws{} &
+      Hchannels_at{_{}}
+    )".
 
   #[global] Instance ws_deques_private_model_timeless t vss :
     Timeless (ws_deques_private_model t vss).
   Proof.
-  Admitted.
+    apply _.
+  Qed.
   #[global] Instance ws_deques_private_inv_persistent t ι sz :
     Persistent (ws_deques_private_inv t ι sz).
   Proof.
-  Admitted.
+    apply _.
+  Qed.
+
+  #[local] Lemma models_alloc sz :
+    ⊢ |==>
+      ∃ γ_models,
+      models_auth' γ_models (replicate sz []) ∗
+      [∗ list] i ∈ seq 0 sz,
+        models_at' γ_models i [].
+  Proof.
+    iMod ghost_list_alloc as "(%γ_models & $ & Hats)".
+    iApply (big_sepL_replicate_1 with "Hats").
+  Qed.
+  #[local] Lemma models_lookup γ vss i vs :
+    models_auth γ vss -∗
+    models_at γ i vs -∗
+    ⌜vss !! i = Some vs⌝.
+  Proof.
+    apply ghost_list_lookup.
+  Qed.
+
+  #[local] Lemma channels_alloc sz :
+    ⊢ |==>
+      ∃ γ_channels,
+      [∗ list] i ∈ seq 0 sz,
+        channels_at' γ_channels i 1 inhabitant.
+  Proof.
+    iAssert (
+      [∗ list] _ ∈ seq 0 sz,
+        |==>
+        ∃ γ_channel,
+        ghost_pred γ_channel (DfracOwn 1) inhabitant
+    )%I as "-#H".
+    { iApply big_sepL_intro. iIntros "!> % % _".
+      iApply ghost_pred_alloc.
+    }
+    iMod (big_sepL_bupd with "H") as "H".
+    iDestruct (big_sepL_exists with "H") as "(%γ_channels & _ & H)".
+    iDestruct (big_sepL2_retract_r with "H") as "(_ & H)".
+    iDestruct (big_sepL_seq_index_2 with "H") as "H".
+    { simpl_length. }
+    iSteps.
+  Qed.
+
+  Opaque channels_at'.
 
   Lemma ws_deques_private_inv_agree t ι sz1 sz2 :
     ws_deques_private_inv t ι sz1 -∗
     ws_deques_private_inv t ι sz2 -∗
     ⌜sz1 = sz2⌝.
   Proof.
-  Admitted.
+    iIntros "(:inv =1) (:inv =2)". simplify.
+    iDestruct (pointsto_agree with "Hl1_size Hl2_size") as %?. naive_solver.
+  Qed.
 
-  Lemma ws_deques_private_inv_owner t ι sz i status :
+  Lemma ws_deques_private_inv_owner t ι sz i status ws :
     ws_deques_private_inv t ι sz -∗
-    ws_deques_private_owner t i status -∗
+    ws_deques_private_owner t i status ws -∗
     ⌜i < sz⌝.
   Proof.
-  Admitted.
-  Lemma ws_deques_private_owner_exclusive t i status1 status2 :
-    ws_deques_private_owner t i status1 -∗
-    ws_deques_private_owner t i status2 -∗
+    iIntros "(:inv) (:owner)". injection Heq as <-.
+    iDestruct (meta_agree with "Hmeta Hmeta_") as %<-.
+    apply lookup_lt_Some in Hdeques_lookup.
+    iSteps.
+  Qed.
+  Lemma ws_deques_private_model_owner t vss i status ws :
+    ws_deques_private_model t vss -∗
+    ws_deques_private_owner t i status ws -∗
+      ∃ vs,
+      ⌜vss !! i = Some vs⌝ ∗
+      ⌜vs `suffix_of` ws⌝.
+  Proof.
+    iIntros "(:model =1) (:owner =2)". simplify.
+    iDestruct (meta_agree with "Hmeta_1 Hmeta_2") as %<-. simplify.
+    iDestruct (models_lookup with "Hmodels_auth Hmodels_at_2") as %Hlookup.
+    iSteps.
+  Qed.
+  Lemma ws_deques_private_owner_exclusive t i status1 ws1 status2 ws2 :
+    ws_deques_private_owner t i status1 ws1 -∗
+    ws_deques_private_owner t i status2 ws2 -∗
     False.
   Proof.
-  Admitted.
+    iIntros "(:owner =1) (:owner =2)". simplify.
+    iDestruct (meta_agree with "Hmeta_1 Hmeta_2") as %<-. simplify.
+    iApply (deque_model_exclusive with "Hdeque_model_1 Hdeque_model_2").
+  Qed.
 
   Lemma ws_deques_private_create_spec ι sz :
     (0 ≤ sz)%Z →
@@ -103,10 +376,66 @@ Section ws_deques_private_G.
       ws_deques_private_inv t ι ₊sz ∗
       ws_deques_private_model t (replicate ₊sz []) ∗
       [∗ list] i ∈ seq 0 ₊sz,
-        ws_deques_private_owner t i Nonblocked
+        ws_deques_private_owner t i Nonblocked []
     }}}.
   Proof.
-  Admitted.
+    iIntros "%Hsz %Φ _ HΦ".
+
+    wp_rec.
+    wp_apply (array_unsafe_make_spec with "[//]") as (responses_array) "Hresponses_model"; first done.
+    iDestruct (array_model_to_inv with "Hresponses_model") as "#Hresponses_inv".
+    wp_apply (array_make_spec with "[//]") as (requests_array) "(_ & Hrequests_model)".
+    iDestruct (array_model_to_inv with "Hrequests_model") as "#Hrequests_inv".
+    wp_apply (array_unsafe_make_spec with "[//]") as (statuses_array) "Hstatuses_model"; first done.
+    iDestruct (array_model_to_inv with "Hstatuses_model") as "#Hstatuses_inv".
+    wp_apply (array_unsafe_init_spec_disentangled (λ _ deque, deque_model deque [])) as (deques_array deques) "(%Hdeques_length & Hdeques_model & Hdeques)"; first done.
+    { iIntros "!> %i %Hi".
+      wp_apply (deque_create_spec with "[//]").
+      iSteps.
+    }
+    iDestruct (array_model_to_inv with "Hdeques_model") as "#Hdeques_inv".
+    iMod (array_model_persist with "Hdeques_model") as "#Hdeques_model".
+    wp_block l as "Hmeta" "(Hl_size & Hl_deques & Hl_statuses & Hl_requests & Hl_responses & _)".
+    iMod (pointsto_persist with "Hl_size") as "#Hl_size".
+    iMod (pointsto_persist with "Hl_deques") as "#Hl_deques".
+    iMod (pointsto_persist with "Hl_statuses") as "#Hl_statuses".
+    iMod (pointsto_persist with "Hl_requests") as "#Hl_requests".
+    iMod (pointsto_persist with "Hl_responses") as "#Hl_responses".
+
+    iMod models_alloc as "(%γ_models & Hmodels_auth & Hmodels_ats)".
+    iMod channels_alloc as "(%γ_channels & Hchannels_ats)".
+
+    pose γ := {|
+      metadata_deques_array := deques_array ;
+      metadata_deques := deques ;
+      metadata_statuses_array := statuses_array ;
+      metadata_requests_array := requests_array ;
+      metadata_responses_array := responses_array ;
+      metadata_inv := ι ;
+      metadata_models := γ_models ;
+      metadata_channels := γ_channels ;
+    |}.
+    iMod (meta_set γ with "Hmeta") as "#Hmeta"; first done.
+
+    iApply "HΦ".
+    iSplitR "Hmodels_auth Hdeques Hmodels_ats Hchannels_ats".
+
+    - rewrite Hdeques_length. simpl_length.
+      iEval (rewrite -(fmap_replicate status_to_val _ Nonblocked)) in "Hstatuses_model".
+      iEval (rewrite -(fmap_replicate request_to_val _ RequestNone)) in "Hrequests_model".
+      iEval (rewrite -(fmap_replicate response_to_val _ ResponseWaiting)) in "Hresponses_model".
+      iExists l, γ. rewrite Z2Nat.id //. iStep 13.
+      iApply inv_alloc. iSteps. iSplitL => /=.
+      + iApply big_sepL_intro. iIntros "!>" (i request (-> & _)%lookup_replicate) "//".
+      + iApply big_sepL_intro. iIntros "!>" (i request (-> & _)%lookup_replicate) "//".
+
+    - iSteps.
+      iDestruct (big_sepL_sep_2 with "Hmodels_ats Hchannels_ats") as "H".
+      iDestruct (big_sepL_to_seq0 with "Hdeques") as "Hdeques". rewrite Hdeques_length.
+      iDestruct (big_sepL_sep_2 with "Hdeques H") as "H".
+      iApply (big_sepL_impl with "H").
+      iSteps.
+  Qed.
 
   Lemma ws_deques_private_size_spec t ι sz :
     {{{
@@ -118,41 +447,45 @@ Section ws_deques_private_G.
       True
     }}}.
   Proof.
-  Admitted.
+    iIntros "%Φ (:inv) HΦ".
 
-  Lemma ws_deques_private_block_spec t ι sz i i_ :
+    wp_rec. wp_load.
+    iSteps.
+  Qed.
+
+ Lemma ws_deques_private_block_spec t ι sz i i_ ws :
     i = ⁺i_ →
     {{{
       ws_deques_private_inv t ι sz ∗
-      ws_deques_private_owner t i_ Nonblocked
+      ws_deques_private_owner t i_ Nonblocked ws
     }}}
       ws_deques_private_block t #i
     {{{
       RET ();
-      ws_deques_private_owner t i_ Blocked
+      ws_deques_private_owner t i_ Blocked ws
     }}}.
   Proof.
   Admitted.
 
-  Lemma ws_deques_private_unblock_spec t ι sz i i_ :
+  Lemma ws_deques_private_unblock_spec t ι sz i i_ ws :
     i = ⁺i_ →
     {{{
       ws_deques_private_inv t ι sz ∗
-      ws_deques_private_owner t i_ Blocked
+      ws_deques_private_owner t i_ Blocked ws
     }}}
       ws_deques_private_unblock t #i
     {{{
       RET ();
-      ws_deques_private_owner t i_ Nonblocked
+      ws_deques_private_owner t i_ Nonblocked ws
     }}}.
   Proof.
   Admitted.
 
-  Lemma ws_deques_private_push_spec t ι sz i i_ v :
+  Lemma ws_deques_private_push_spec t ι sz i i_ ws v :
     i = ⁺i_ →
     <<<
       ws_deques_private_inv t ι sz ∗
-      ws_deques_private_owner t i_ Nonblocked
+      ws_deques_private_owner t i_ Nonblocked ws
     | ∀∀ vss,
       ws_deques_private_model t vss
     >>>
@@ -162,43 +495,45 @@ Section ws_deques_private_G.
       ⌜vss !! i_ = Some vs⌝ ∗
       ws_deques_private_model t (<[i_ := vs ++ [v]]> vss)
     | RET ();
-      ws_deques_private_owner t i_ Nonblocked
+      ws_deques_private_owner t i_ Nonblocked (vs ++ [v])
     >>>.
   Proof.
   Admitted.
 
-  Lemma ws_deques_private_pop_spec t ι sz i i_ :
+  Lemma ws_deques_private_pop_spec t ι sz i i_ ws :
     i = ⁺i_ →
     <<<
       ws_deques_private_inv t ι sz ∗
-      ws_deques_private_owner t i_ Nonblocked
+      ws_deques_private_owner t i_ Nonblocked ws
     | ∀∀ vss,
       ws_deques_private_model t vss
     >>>
       ws_deques_private_pop t #i @ ↑ι
     <<<
-      ∃∃ o,
+      ∃∃ o ws,
       match o with
       | None =>
           ⌜vss !! i_ = Some []⌝ ∗
+          ⌜ws = []⌝ ∗
           ws_deques_private_model t vss
       | Some v =>
           ∃ vs,
           ⌜vss !! i_ = Some (vs ++ [v])⌝ ∗
+          ⌜ws = vs ++ [v]⌝ ∗
           ws_deques_private_model t (<[i_ := vs]> vss)
       end
     | RET o;
-      ws_deques_private_owner t i_ Nonblocked
+      ws_deques_private_owner t i_ Nonblocked ws
     >>>.
   Proof.
   Admitted.
 
-  Lemma ws_deques_private_steal_to_spec t ι (sz : nat) i i_ j :
+  Lemma ws_deques_private_steal_to_spec t ι (sz : nat) i i_ ws j :
     i = ⁺i_ →
     (0 ≤ j < sz)%Z →
     <<<
       ws_deques_private_inv t ι sz ∗
-      ws_deques_private_owner t i_ Blocked
+      ws_deques_private_owner t i_ Blocked ws
     | ∀∀ vss,
       ws_deques_private_model t vss
     >>>
@@ -214,17 +549,86 @@ Section ws_deques_private_G.
           ws_deques_private_model t (<[₊j := vs]> vss)
       end
     | RET o;
-      ws_deques_private_owner t i_ Blocked
+      ws_deques_private_owner t i_ Blocked ws
     >>>.
   Proof.
   Admitted.
+End ws_deques_private_G.
 
-  Lemma ws_deques_private_steal_as_spec t ι sz i i_ round :
+#[global] Opaque ws_deques_private_inv.
+#[global] Opaque ws_deques_private_model.
+#[global] Opaque ws_deques_private_owner.
+
+Section ws_deques_private_G.
+  Context `{ws_deques_private_G : WsDequesPrivateG Σ}.
+
+  #[local] Lemma ws_deques_private_steal_as_0_spec t ι (sz : nat) i i_ ws round (n : nat) :
+    i = ⁺i_ →
+    <<<
+      ws_deques_private_inv t ι sz ∗
+      ws_deques_private_owner t i_ Blocked ws ∗
+      random_round_model' round (sz - 1) n
+    | ∀∀ vss,
+      ws_deques_private_model t vss
+    >>>
+      ws_deques_private_steal_as_0 t #sz #i round #n @ ↑ι
+    <<<
+      ∃∃ o,
+      match o with
+      | None =>
+          ws_deques_private_model t vss
+      | Some v =>
+          ∃ j vs,
+          ⌜₊i ≠ j⌝ ∗
+          ⌜vss !! j = Some (v :: vs)⌝ ∗
+          ws_deques_private_model t (<[j := vs]> vss)
+      end
+    | RET o;
+      ∃ n,
+      ws_deques_private_owner t i_ Blocked ws ∗
+      random_round_model' round (sz - 1) n
+    >>>.
+  Proof.
+    iIntros (->) "%Φ (#Hinv & Howner & Hround) HΦ".
+    iDestruct (ws_deques_private_inv_owner with "Hinv Howner") as %Hi.
+
+    iLöb as "HLöb" forall (n).
+
+    wp_rec. wp_pures.
+    case_bool_decide as Hcase; wp_pures.
+
+    - iMod "HΦ" as "(%vss & Hmodel & _ & HΦ)".
+      iApply ("HΦ" $! None with "Hmodel [$Howner Hround]"); first iSteps.
+
+    - wp_apply (random_round_next_spec' with "Hround") as (j) "(%Hj & Hround)"; first lia.
+      wp_pures.
+      rewrite Nat2Z.id.
+      pose k := (i_ + 1 + j) `mod` sz.
+      assert ((i_ + 1 + j) `rem` sz = k)%Z as ->.
+      { rewrite Z.rem_mod_nonneg; lia. }
+      awp_smart_apply (ws_deques_private_steal_to_spec with "[$Hinv $Howner]") without "Hround"; [done | lia |].
+      iApply (aacc_aupd with "HΦ"); first done. iIntros "%vss Hmodel".
+      iAaccIntro with "Hmodel"; first iSteps. iIntros ([ v |]).
+
+      + rewrite Nat2Z.id.
+        iSteps as (vs Hlookup) "Hmodel". iExists (Some v). iSteps. iExists k. iSteps. iPureIntro.
+        clear Hlookup. rewrite {}/k.
+        destruct (decide (i_ + 1 + j < sz)).
+        * rewrite Nat.mod_small //. lia.
+        * assert (i_ + 1 + j < sz * 2) as ?%Nat.div_lt_upper_bound by lia; last lia.
+          assert ((i_ + 1 + j) `div` sz = 1) by lia.
+          lia.
+
+      + iSteps as "HΦ Howner Hround".
+        assert (n - 1 = (n - 1)%nat)%Z as -> by lia.
+        iSteps.
+  Qed.
+  Lemma ws_deques_private_steal_as_spec t ι sz i i_ ws round :
     i = ⁺i_ →
     0 < sz →
     <<<
       ws_deques_private_inv t ι sz ∗
-      ws_deques_private_owner t i_ Blocked ∗
+      ws_deques_private_owner t i_ Blocked ws ∗
       random_round_model' round (sz - 1) (sz - 1)
     | ∀∀ vss,
       ws_deques_private_model t vss
@@ -243,11 +647,18 @@ Section ws_deques_private_G.
       end
     | RET o;
       ∃ n,
-      ws_deques_private_owner t i_ Blocked ∗
+      ws_deques_private_owner t i_ Blocked ws ∗
       random_round_model' round (sz - 1) n
     >>>.
   Proof.
-  Admitted.
+    iIntros (->) "%Hsz %Φ (#Hinv & Hround) HΦ".
+
+    wp_rec.
+    wp_smart_apply (ws_deques_private_size_spec with "Hinv") as "_".
+    wp_pures.
+    assert (sz - 1 = (sz - 1)%nat)%Z as -> by lia.
+    wp_apply (ws_deques_private_steal_as_0_spec with "[$Hinv $Hround] HΦ"); first done.
+  Qed.
 End ws_deques_private_G.
 
 #[global] Opaque ws_deques_private_create.
@@ -258,7 +669,3 @@ End ws_deques_private_G.
 #[global] Opaque ws_deques_private_pop.
 #[global] Opaque ws_deques_private_steal_to.
 #[global] Opaque ws_deques_private_steal_as.
-
-#[global] Opaque ws_deques_private_inv.
-#[global] Opaque ws_deques_private_model.
-#[global] Opaque ws_deques_private_owner.
